src/core/examples/STTT16/sttt_example.thy
@@ -4,10 +4,19 @@ begin
 section "the dist example"
 thm conj_disj_distribR ex_disj_distrib
 
+ML{*-
+  TextSocket.safe_close();
+*} 
+
 lemma "\<exists>x y. (x = y \<or> x > y) \<and> (x*x + y*y = (50::nat))"
 (*apply (subst conj_disj_distribR)
 apply (subst ex_disj_distrib)+*)
 apply (tinker disj)
+ML_val {*-
+  val st =  Thm.cprem_of (#goal @{Isar.goal}) 1 |> Thm.term_of;
+  val ps_thm = Tinker.start_ieval @{context} (SOME disj) (SOME []) (SOME st) (* prove the goal *)
+          |> EData.get_pplan |> IsaProver.get_goal_thm(* get the theorem *)
+*}
 apply (rule disjI1)
 apply (rule_tac x = 5 in exI)+
 by simp
@@ -29,41 +38,20 @@ lemma running_example: "callee = Domain(call :: Digitseq rel) \<Longrightarrow>
        \<exists> callee' call'. (\<forall> x y. y \<in> call' `` {x} \<longrightarrow> x \<noteq> y) \<and>
          (callee' = Domain call') \<and> call' = call \<union> {(s1, s2)} "
 apply (tinker onep)
-ML_val {*- 
+ML_val {*-
   val st =  Thm.cprem_of (#goal @{Isar.goal}) 1 |> Thm.term_of;
-  val ps_thm = Tinker.start_ieval @{context} (SOME onep0) (SOME []) (SOME st) (* prove the goal *)
+  val ps_thm = Tinker.start_ieval @{context} (SOME onep) (SOME []) (SOME st) (* prove the goal *)
           |> EData.get_pplan |> IsaProver.get_goal_thm(* get the theorem *)
 *}
 (* some intermediate steps to simp goals *)
 apply (intro conjI) prefer 2 apply (rule refl) prefer 2 apply (rule refl) 
-
-apply (tinker rippling)
-ML_val {*-
+(*apply (tinker rippling)*)
+ML_val {*- 
   val st =  Thm.cprem_of (#goal @{Isar.goal}) 1 |> Thm.term_of;
   val ps_thm = Tinker.start_ieval @{context} (SOME rippling) (SOME []) (SOME st) (* prove the goal *)
           |> EData.get_pplan |> IsaProver.get_goal_thm(* get the theorem *)
 *}
-
-
-
-find_theorems "(_ \<or> _)\<longrightarrow>_"
-thm Relation.Domain_Un_eq  Set.Un_iff Relation.Un_Image
-HOL.conj_disj_distribL HOL.conj_disj_distribR HOL.imp_disjL
-apply (subst Relation.Un_Image)
-apply (subst Set.Un_iff)+
-apply (subst HOL.imp_disjL)
-
-(* end of rippling, now pwf *)
-apply (intro allI) apply(erule_tac x = x in allE) apply(erule_tac x = y in allE)
-(* end of pwf forall *)
-apply (rule conjI)
-(*fertilisation*)
-apply (simp only:)
-(* auto *)
-apply simp
-ML{*-
-  TextSocket.safe_close();
-*} 
+done
 
 
 
